DynamoDbEncryptionMiddlewareInternal/src/TransactWriteItemsTransform.dfy
@@ -28,13 +28,12 @@ module TransactWriteItemsTransform {
     ensures output.Success? ==> |output.value.transformedInput.TransactItems| == |input.sdkInput.TransactItems|
 
     //= specification/dynamodb-encryption-client/ddb-sdk-integration.md#encrypt-before-transactwriteitems
-    //= type=implication
     //# To protect against a possible fifth field being added to the TransactWriteItem structure in the future,
     //# the client MUST fail if none of the `Update`, `ConditionCheck`, `Delete` and `Put` fields are set.
     ensures output.Success? ==>
       forall item <- input.sdkInput.TransactItems :: IsValid(item)
   {
-    :- Need(forall item <- input.sdkInput.TransactItems :: IsValid(item), E("Each item in TransactWriteItems must specify at least one operation"));
+    :- Need(forall item <- input.sdkInput.TransactItems :: IsValid(item), E("Each item in TransactWriteItems must specify at least one supported operation"));
     var result : seq<DDB.TransactWriteItem> := [];
     for x := 0 to |input.sdkInput.TransactItems|
       invariant |result| == x
@@ -110,7 +109,8 @@ module TransactWriteItemsTransform {
         //# the result [Encrypted DynamoDB Item](./encrypt-item.md#encrypted-dynamodb-item)
         //# calculated above.
         var put := Some(item.Put.value.(Item := encrypted.encryptedItem));
-        result := result + [item.(Put := put)];
+        var newItem := item.(Put := put);
+        result := result + [newItem];
       } else {
         //= specification/dynamodb-encryption-client/ddb-sdk-integration.md#encrypt-before-transactwriteitems
         //# Any actions other than `Put, MUST be unchanged.
